src/automation.v
@@ -130,27 +130,6 @@ Proof.
   autounfold with tla; intuition auto.
 Qed.
 
-Lemma combine_preds (next: Σ → Σ → Prop) (P: Σ → Prop) :
-  (□ ⟨ next ⟩ ∧ □ ⌜ P ⌝) == □ ⟨ λ s s', next s s' ∧ P s ∧ P s' ⟩.
-Proof.
-  unseal.
-  intuition eauto.
-  - specialize (H k). intuition auto.
-  - specialize (H k). intuition auto.
-Qed.
-
-Lemma combine_state_preds (P Q: Σ → Prop) :
-  (⌜P⌝ ∧ ⌜Q⌝) == ⌜λ s, P s ∧ Q s⌝.
-Proof.
-  unseal.
-Qed.
-
-Lemma not_state_pred (P: Σ → Prop) :
-  !⌜λ s, P s⌝ == ⌜λ s, ¬ P s⌝.
-Proof.
-  unseal.
-Qed.
-
 End TLA.
 
 Hint Rewrite not_eventually not_always
@@ -250,7 +229,7 @@ Ltac tla_pose lem :=
   let H := fresh "Htemp" in
   epose proof lem as H;
   apply (tla_pose_lemma _ _ H); clear H;
-  [ tla_prop | rewrite tla_and_assoc ].
+  [ tla_prop | try rewrite tla_and_assoc ].
 
 Ltac tla_split :=
   match goal with
